proof/xkem_avx2_clean.ec
@@ -75,6 +75,7 @@ module M = {
     var sk_mlkem:W8.t Array2400.t;
     var i:int;
     var t64:W64.t;
+    var  _0: W64.t;
     expanded <- witness;
     expanded_mlkem <- witness;
     expanded_x25519 <- witness;
@@ -101,10 +102,11 @@ module M = {
     (Array32.init (fun i_0 => expanded.[((32 + 32) + i_0)]));
     pk_x25519 <@ xwing_x25519_base (pk_x25519, expanded_x25519);
     expanded_mlkem <- (Array64.init (fun i_0 => expanded.[(0 + i_0)]));
-    (pk_mlkem, sk_mlkem) <@ Jkem_avx2_stack.M.__crypto_kem_keypair_jazz (pk_mlkem, sk_mlkem, expanded_mlkem);
+    (pk_mlkem, sk_mlkem, _0) <@ Jkem_avx2_stack.M.jade_kem_mlkem_mlkem768_amd64_avx2_keypair_derand(pk_mlkem, sk_mlkem, expanded_mlkem);
     (* Erased call to unspill *)
+    aux <- (((3 * 384) + 32) %/ 8);
     i <- 0;
-    while ((i < 148)) {
+    while ((i < aux)) {
       t64 <- (get64 (WArray1184.init8 (fun i_0 => pk_mlkem.[i_0])) i);
       pkp <-
       (Array1216.init
@@ -113,8 +115,9 @@ module M = {
       i <- (i + 1);
     }
 
+    aux <- (32 %/ 8);
     i <- 0;
-    while ((i < 4)) {
+    while ((i < aux)) {
       t64 <- (get64 (WArray32.init8 (fun i_0 => pk_x25519.[i_0])) i);
       pkp <-
       (Array1216.init
@@ -123,8 +126,10 @@ module M = {
       ((((3 * 384) + 32) %/ 8) + i) t64)));
       i <- (i + 1);
     }
+
+    aux <- (32 %/ 8);
     i <- 0;
-    while ((i < 4)) {
+    while ((i < aux)) {
       t64 <- (get64 (WArray32.init8 (fun i_0 => srandomness.[i_0])) i);
       skp <-
       (Array32.init
@@ -195,8 +200,9 @@ module M = {
     ss <@ _sha3_256_A128__A6 (ss, ss_mlkem, ss_x25519, ct_x25519, pk_x25519);
     (* Erased call to unspill *)
 
+    aux <- (((3 * 320) + 128) %/ 8);
     i <- 0;
-    while ((i < 136)) {
+    while ((i < aux)) {
       t64 <- (get64 (WArray1088.init8 (fun i_0 => ct_mlkem.[i_0])) i);
       ctp <-
       (Array1120.init
@@ -204,8 +210,10 @@ module M = {
       (WArray1120.set64 (WArray1120.init8 (fun i_0 => ctp.[i_0])) i t64)));
       i <- (i + 1);
     }
+
+    aux <- (32 %/ 8);
     i <- 0;
-    while ((i < 4)) {
+    while ((i < aux)) {
       t64 <- (get64 (WArray32.init8 (fun i_0 => ct_x25519.[i_0])) i);
       ctp <-
       (Array1120.init
@@ -215,8 +223,9 @@ module M = {
       i <- (i + 1);
     }
 
+    aux <- (32 %/ 8);
     i <- 0;
-    while ((i < 4)) {
+    while ((i < aux)) {
       t64 <- (get64 (WArray32.init8 (fun i_0 => ss.[i_0])) i);
       shkp <-
       (Array32.init
@@ -295,8 +304,9 @@ module M = {
     ss <@ _sha3_256_A128__A6 (ss, ss_mlkem, ss_x25519, ct_x25519, pk_x25519);
     (* Erased call to unspill *)
 
+    aux <- (32 %/ 8);
     i <- 0;
-    while ((i < 4)) {
+    while ((i < aux)) {
       t64 <- (get64 (WArray32.init8 (fun i_0 => ss.[i_0])) i);
       shkp <-
       (Array32.init
